Breaking out State into its own file

src/Assembly/QhasmCommon.v
@@ -1,36 +1,10 @@
-Require Export String List Logic.
+Require Export String List.
 Require Export Bedrock.Word.
 
-Require Import ZArith NArith NPeano.
-Require Import Coq.Structures.OrderedTypeEx.
-Require Import FMapAVL FMapList.
-Require Import JMeq.
-
-Require Import QhasmUtil.
-
-Import ListNotations.
-
-Module NatM := FMapAVL.Make(Nat_as_OT).
-Definition DefMap: Type := NatM.t N.
-Definition StateMap: Type := NatM.t DefMap.
-Definition LabelMap: Type := NatM.t nat.
-
-(* Sugar *)
-
-Definition W := word 32.
-
-Definition convert {A B: Type} (x: A) (H: A = B): B :=
- eq_rect A (fun B0 : Type => B0) x B H.
-
-Ltac create X Y :=
-  let H := fresh in (
-    assert (exists X, X = Y) as H
-      by (exists Y; abstract intuition);
-    destruct H).
-
-Obligation Tactic := abstract intuition.
-
 (* A formalization of x86 qhasm *)
+Definition Label := nat.
+Definition Index (limit: nat) := {x: nat | (x < limit)%nat}.
+Definition Invert := bool.
 
 (* A constant upper-bound on the number of operations we run *)
 Definition maxOps: nat := 1000.
@@ -131,11 +105,6 @@ Definition invertConditional (c: Conditional): Conditional :=
 
 Hint Constructors Conditional.
 
-(* Machine State *)
-
-Inductive State :=
-| fullState (regState: StateMap) (stackState: DefMap): State.
-
 (* Reg, Stack, Const Utilities *)
 
 Definition getRegWords {n} (x: Reg n) :=
@@ -171,167 +140,6 @@ Definition getStackIndex {n} (x: Stack n): nat :=
   | stack256 loc => loc
   | stack512 loc => loc
   end.
-
-(* State Manipulations *)
-
-Definition getReg {n} (reg: Reg n) (state: State): option (word n) :=
-  match state with
-  | fullState regState stackState =>
-    match (NatM.find n regState) with
-      | Some map =>
-        match (NatM.find (getRegIndex reg) map) with
-        | Some m => Some (NToWord n m)
-        | _ => None
-        end
-      | None => None
-    end
-  end.
-
-Definition setReg {n} (reg: Reg n) (value: word n) (state: State): option State :=
-  match state with
-  | fullState regState stackState =>
-    match (NatM.find n regState) with
-      | Some map =>
-        Some (fullState
-          (NatM.add n (NatM.add (getRegIndex reg) (wordToN value) map)
-            regState) stackState)
-      | None => None
-    end
-  end.
-
-(* Per-word Stack Operations *)
-Definition getStack32 (entry: Stack 32) (state: State): option (word 32) :=
-  match state with
-  | fullState regState stackState =>
-    match entry with
-    | stack32 loc =>
-      match (NatM.find loc stackState) with
-      | Some n => Some (NToWord 32 n)
-      | _ => None
-      end
-    end
-  end.
-
-Definition setStack32 (entry: Stack 32) (value: word 32) (state: State): option State :=
-  match state with
-  | fullState regState stackState =>
-    match entry with
-    | stack32 loc =>
-      (Some (fullState regState
-                       (NatM.add loc (wordToN value) stackState)))
-    end
-  end.
-
-Notation "'cast' e" := (convert e _) (at level 20).
-
-(* Iterating Stack Operations *)
-Lemma getStackWords_spec: forall {n} (x: Stack n), n = 32 * (getStackWords x).
-Proof. intros; destruct x; simpl; intuition. Qed.
-
-Definition segmentStackWord {n} (x: Stack n) (w: word n): word (32 * (getStackWords x)).
-  intros; destruct x; simpl; intuition.
-Defined.
-
-Definition desegmentStackWord {n} (x: Stack n) (w: word (32 * (getStackWords x))): word n.
-  intros; destruct x; simpl; intuition.
-Defined.
-
-Inductive Either A B := | xleft: A -> Either A B | xright: B -> Either A B.
-
-Definition getWords' {n} (st: (list (word 32)) * word (32 * n)) :
-    Either (list (word 32)) ((list (word 32)) * word (32 * (n - 1))).
-
-  destruct (Nat.eq_dec n 0) as [H | H];
-    destruct st as [lst w].
-
-  - refine (xleft _ _ lst).
-
-  - refine (xright _ _
-             (cons (split1 32 (32 * (n - 1)) (cast w)) lst,
-             (split2 32 (32 * (n - 1)) (cast w)))); intuition.
-Defined.
-
-Program Fixpoint getWords'_iter (n: nat) (st: (list (word 32)) * word (32 * n)): list (word 32) :=
-  match n with
-  | O => fst st
-  | S m =>
-    match (getWords' st) with
-    | xleft lst => lst
-    | xright st => cast (getWords'_iter m st)
-    end
-  end.
-
-Definition getWords {len} (wd: word (32 * len)): list (word 32) :=
-  getWords'_iter len ([], wd).
-
-Definition joinWordOpts_expandTerm {n} (w: word (32 + 32 * n)): word (32 * S n).
-  replace (32 * S n) with (32 + 32 * n) by abstract intuition; assumption.
-Defined.
-
-Fixpoint joinWordOpts (wds: list (option (word 32))) (len: nat): option (word (32 * (length wds))).
-  refine match len with
-  | O => None
-  | S len' =>
-    match wds with
-    | nil => None
-    | (cons wo wos) =>
-        match wo with
-        | None => None
-        | Some w =>
-          let f := fun x =>
-            match x with 
-            | None => None
-            | (Some joined) => Some (cast (combine w joined))
-            end in
-
-          f (joinWordOpts wos len')
-        end
-    end
-  end; 
-    try replace (Datatypes.length (wo :: wos))
-           with (1 + (Datatypes.length wos))
-             by abstract intuition;
-    intuition.
-Defined.
-
-Definition setStack {n} (entry: Stack n) (value: word n) (state: State) : option State :=
-  (fix setStack_iter (wds: list (word 32)) (nextLoc: nat) (state: State) :=
-     match wds with
-     | [] => Some state
-     | w :: ws =>
-       match (setStack32 (stack32 nextLoc) w state) with 
-       | Some st' => setStack_iter ws (S nextLoc) st'
-       | None => None
-       end
-     end) (getWords (segmentStackWord entry value)) (getStackIndex entry) state.
-
-Fixpoint getStack_iter (rem: nat) (loc: nat) (state: State): list (option (word 32)) :=
-  match rem with
-  | O => []
-  | (S rem') =>
-    (getStack32 (stack32 loc) state) ::
-      (getStack_iter rem' (loc + 32) state)
-  end.
-
-Fixpoint getStack {n} (entry: Stack n) (state: State) : option (word n).
-  refine (
-    let m := getStackWords entry in
-    let i := getStackIndex entry in
-    let wos := (getStack_iter m i state) in
-    let joined := (joinWordOpts wos) in
-    option_map (fun a => cast a) joined
-  ); intuition.
-
-  replace (Datatypes.length _) with (getStackWords entry); intuition.
-  unfold wds.
-  induction (getStackWords entry); simpl; intuition.
-  destruct entry.
-
-  simpl; intuition.
-Defined.
-
-Definition emptyState: State :=
-  fullState (NatM.empty DefMap) (NatM.empty DefMap).
 
 (* For register allocation checking *)
 Definition regCount (base: nat): nat :=
