src/Assembly/State.v
@@ -1,0 +1,216 @@
+Require Export String List Logic.
+Require Export Bedrock.Word.
+
+Require Import ZArith NArith NPeano.
+Require Import Coq.Structures.OrderedTypeEx.
+Require Import FMapAVL FMapList.
+Require Import JMeq.
+
+Require Import QhasmUtil QhasmCommon.
+
+(* There's a lot in here.
+   We don't want to automatically give it all to the client. *)
+
+Module State.
+    Import ListNotations.
+    Import Util.
+
+    Module NatM := FMapAVL.Make(Nat_as_OT).
+    Definition DefMap: Type := NatM.t N.
+    Definition StateMap: Type := NatM.t DefMap.
+    Definition LabelMap: Type := NatM.t nat.
+
+    Delimit Scope state_scope with state.
+    Local Open Scope state_scope.
+
+    (* Sugar and Tactics *)
+
+    Definition convert {A B: Type} (x: A) (H: A = B): B :=
+    eq_rect A (fun B0 : Type => B0) x B H.
+
+    Notation "'always' A" := (fun _ => A) (at level 90) : state_scope.
+    Notation "'cast' e" := (convert e _) (at level 20) : state_scope.
+    Notation "'lift' e" := (exist _ e _) (at level 20) : state_scope.
+    Notation "'contra'" := (False_rec _ _) : state_scope.
+
+    Obligation Tactic := abstract intuition.
+
+    (* The Big Definition *)
+
+    Inductive State :=
+      | fullState (regState: StateMap) (stackState: DefMap): State.
+
+    Definition emptyState: State := fullState (NatM.empty DefMap) (NatM.empty N).
+
+    (* Register State Manipulations *)
+
+    Definition getReg {n} (reg: Reg n) (state: State): option (word n) :=
+      match state with
+      | fullState regState stackState =>
+        match (NatM.find n regState) with
+        | Some map =>
+            match (NatM.find (getRegIndex reg) map) with
+            | Some m => Some (NToWord n m)
+            | _ => None
+            end
+        | None => None
+        end
+      end.
+
+    Definition setReg {n} (reg: Reg n) (value: word n) (state: State): option State :=
+      match state with
+      | fullState regState stackState =>
+        match (NatM.find n regState) with
+        | Some map =>
+            Some (fullState
+                    (NatM.add n (NatM.add (getRegIndex reg) (wordToN value) map) regState)
+                    stackState)
+        | None => None
+        end
+      end.
+
+    (* Per-word Stack Operations *)
+
+    Definition getStack32 (entry: Stack 32) (state: State): option (word 32) :=
+      match state with
+      | fullState regState stackState =>
+        match entry with
+        | stack32 loc =>
+          match (NatM.find loc stackState) with
+          | Some n => Some (NToWord 32 n)
+          | _ => None
+          end
+        end
+      end.
+
+    Definition setStack32 (entry: Stack 32) (value: word 32) (state: State): option State :=
+    match state with
+    | fullState regState stackState =>
+        match entry with
+        | stack32 loc =>
+        (Some (fullState regState
+              (NatM.add loc (wordToN value) stackState)))
+        end
+    end.
+
+    (* Inductive Word Manipulations*)
+
+    Definition getWords' {n} (st: (list (word 32)) * word (32 * n)) :
+        Either (list (word 32)) ((list (word 32)) * word (32 * (n - 1))).
+
+      destruct (Nat.eq_dec n 0) as [H | H];
+        destruct st as [lst w].
+
+    - refine (xleft _ _ lst).
+
+    - refine (xright _ _
+             (cons (split1 32 (32 * (n - 1)) (cast w)) lst,
+             (split2 32 (32 * (n - 1)) (cast w))));
+      intuition.
+    Defined.
+
+    Program Fixpoint getWords'_iter (n: nat) (st: (list (word 32)) * word (32 * n)): list (word 32) :=
+      match n with
+      | O => fst st
+      | S m =>
+        match (getWords' st) with
+        | xleft lst => lst
+        | xright st => cast (getWords'_iter m st)
+        end
+      end.
+
+    Definition getWords {len} (wd: word (32 * len)): list (word 32) :=
+      getWords'_iter len ([], wd).
+
+    Definition joinWordOpts_expandTerm {n} (w: word (32 + 32 * n)): word (32 * S n).
+      replace (32 * S n) with (32 + 32 * n) by abstract intuition; assumption.
+    Defined.
+
+    Fixpoint joinWordOpts'
+            (len: nat)
+            (rem: nat)
+            (wds: list (option (word 32)))
+            (cont: word (32 * (len - rem)))
+        : (rem <= len)%nat -> (length wds = rem) -> option (word (32 * len)).
+
+      refine (fun remCorrect wdsCorrect =>
+      match rem as r return r = rem -> _ with
+      | O => always Some (cast cont)
+      | (S rem') => always
+        match wds as l return l = wds -> _ with
+        | nil => always None
+        | (cons wo wos) => always
+            match wo with
+            | None => None
+            | Some w => (joinWordOpts' len rem' wos (cast (combine w cont)) _ _)
+            end
+        end (eq_refl wds)
+      end (eq_refl rem)); intuition.
+
+      rewrite <- _H in wdsCorrect; rewrite <- _H0 in *;
+        replace (length (wo::wos)) with (1 + length wos) in wdsCorrect by abstract intuition;
+        intuition.
+
+    Admitted.
+
+    Definition joinWordOpts (wds: list (option (word 32))): option (word (32 * (length wds))).
+      refine (joinWordOpts' (length wds) (length wds) wds (cast (wzero 0)) _ _); intuition.
+    Defined.
+
+    (* Stack Manipulations *)
+
+    Fixpoint getStack_iter (rem: nat) (loc: nat) (state: State): list (option (word 32)) :=
+      match rem with
+      | O => []
+      | (S rem') =>
+        (getStack32 (stack32 loc) state) ::
+        (getStack_iter rem' (loc + 32) state)
+    end.
+
+    Lemma getStack_iter_length: forall rem loc state,
+        length (getStack_iter rem loc state) = rem.
+    Proof.
+      induction rem; intuition.
+
+      replace (getStack_iter (S rem) loc state) with 
+        ((getStack32 (stack32 loc) state) ::
+        (getStack_iter rem (loc + 32) state)) by intuition.
+
+      replace (Datatypes.length _) with
+        (1 + Datatypes.length (getStack_iter rem (loc + 32) state)) by intuition.
+
+      rewrite IHrem; intuition.
+    Qed.
+
+    Fixpoint getStack {n} (entry: Stack n) (state: State) : option (word n).
+
+      refine (
+        let m := getStackWords entry in
+        let i := getStackIndex entry in
+        let wos := (getStack_iter m i state) in
+        let joined := (joinWordOpts wos) in
+
+        match joined as j return j = joined -> _ with
+        | Some w => always Some (cast w)
+        | None => always None
+        end (eq_refl joined)
+      ); abstract (
+        intuition;
+        unfold wos;
+        rewrite getStack_iter_length;
+        destruct entry; simpl; intuition).
+
+    Admitted.
+
+    Definition setStack {n} (entry: Stack n) (value: word n) (state: State) : option State :=
+      (fix setStack_iter (wds: list (word 32)) (nextLoc: nat) (state: State) :=
+        match wds with
+        | [] => Some state
+        | w :: ws =>
+        match (setStack32 (stack32 nextLoc) w state) with 
+        | Some st' => setStack_iter ws (S nextLoc) st'
+        | None => None
+        end
+        end) (getWords (segmentStackWord entry value)) (getStackIndex entry) state.
+
+End State.
